done/Iron/Language/SystemF2Data/Type/Base.v
@@ -1,38 +1,7 @@
 
 Require Export Iron.Language.SystemF2Data.Base.
 Require Export Iron.Language.SystemF2Data.Kind.
-
-
-(********************************************************************)
-(* Type Constructors. *)
-Inductive tycon : Type :=
- | TyConFun  : tycon
- | TyConData : nat   -> ki -> tycon.
-Hint Constructors tycon.
-
-
-Fixpoint tycon_beq t1 t2 :=
- match t1, t2 with
- | TyConFun,       TyConFun       => true
- | TyConData n1 _, TyConData n2 _ => beq_nat n1 n2
- | _,              _              => false
- end.
-
-
-Definition isTyConFun  (tc: tycon) : Prop :=
- match tc with
- | TyConFun      => True
- | TyConData _ _ => False
- end.
-Hint Unfold isTyConFun.
-
-
-Definition isTyConData (tc: tycon) : Prop :=
- match tc with
- | TyConFun      => False
- | TyConData _ _ => True
- end.
-Hint Unfold isTyConData.
+Require Export Iron.Language.SystemF2Data.Type.TyCon.
 
 
 (********************************************************************)
