done/Iron/Language/SystemF2Data/Type/TyCon.v
@@ -1,0 +1,45 @@
+
+Require Export Iron.Language.SystemF2Data.Base.
+Require Export Iron.Language.SystemF2Data.Kind.
+
+
+(* Type Constructors. *)
+Inductive tycon : Type :=
+ (* The function type constructor. *)
+ | TyConFun  : tycon
+
+ (* Primitive type constructors. *)
+ | TyConNat  : tycon
+ | TyConBool : tycon
+
+ (* Data type constructors. *)
+ | TyConData : nat   -> ki -> tycon.
+Hint Constructors tycon.
+
+
+(* Check whether two type constructors are equal. *)
+Fixpoint tycon_beq t1 t2 :=
+ match t1, t2 with
+ | TyConFun,       TyConFun       => true
+ | TyConNat,       TyConNat       => true
+ | TyConBool,      TyConBool      => true
+ | TyConData n1 _, TyConData n2 _ => beq_nat n1 n2
+ | _,              _              => false
+ end.
+
+
+Definition isTyConFun  (tc: tycon) : Prop :=
+ match tc with
+ | TyConFun      => True
+ | _             => False
+ end.
+Hint Unfold isTyConFun.
+
+
+Definition isTyConData (tc: tycon) : Prop :=
+ match tc with
+ | TyConData _ _ => True
+ | _             => False
+ end.
+Hint Unfold isTyConData.
+
